compiler/backend/clos_callScript.sml
@@ -228,7 +228,7 @@ val compile_LENGTH = Q.store_thm("compile_LENGTH",
   \\ imp_res_tac calls_length \\ rw[]);
 
 val compile_nil = Q.store_thm("compile_nil",
-  `clos_call$compile x [] = (a,b) ⇒ a =[] ∧ b = []`,
+  `clos_call$compile x [] = (a,g,b) ⇒ a =[] ∧ g = LN ∧ b = []`,
   Cases_on`x` \\ rw[compile_def]
   \\ pairarg_tac \\ fs[] \\ fs[calls_def] \\ rw[]);
 
